veric/tycontext.v
@@ -310,57 +310,6 @@ Definition composite_env_legal_fieldlist env :=
   forall (id : positive) (co : composite),
     env ! id = Some co -> composite_legal_fieldlist co.
 
-Section cuof.
-
-Context (cenv: composite_env).
-
-Fixpoint complete_legal_cosu_type t :=
-  match t with
-  | Tarray t' _ _ => complete_legal_cosu_type t'
-  | Tstruct id _ => match cenv ! id with
-                    | Some co => match co_su co with
-                                 | Struct => true
-                                 | Union => false
-                                 end
-                    | _ => false
-                    end
-  | Tunion id _ => match cenv ! id with
-                   | Some co => match co_su co with
-                                | Struct => false
-                                | Union => true
-                                end
-                   | _ => false
-                   end
-  | Tfunction _ _ _
-  | Tvoid => false
-  | _ => true
-  end.
-
-Fixpoint composite_complete_legal_cosu_type (m: members): bool :=
-  match m with
-  | nil => true
-  | (_, t) :: m' => complete_legal_cosu_type t && composite_complete_legal_cosu_type m'
-  end.
-
-Definition composite_env_complete_legal_cosu_type: Prop :=
-  forall (id : positive) (co : composite),
-    cenv ! id = Some co -> composite_complete_legal_cosu_type (co_members co) = true.
-  
-End cuof.
-
-Lemma complete_legal_cosu_type_complete_type: forall cenv: composite_env,
-  forall t,
-    complete_legal_cosu_type cenv t = true ->
-    complete_type cenv t = true.
-Proof.
-  intros.
-  induction t; auto.
-  + simpl in *.
-    destruct (cenv ! i); auto.
-  + simpl in *.
-    destruct (cenv ! i); auto.
-Qed.
-
 Class compspecs := mkcompspecs {
   cenv_cs : composite_env;
   cenv_consistent: composite_env_consistent cenv_cs;
